src/proofs/bn_axioms.dfy
@@ -1,0 +1,39 @@
+include "../common/commons.dfy"
+
+module Block_BN_Axioms
+{
+    import opened Types 
+    import opened CommonFunctions
+
+    datatype BNState = BNState(
+        state_roots_of_imported_blocks: set<Root>,
+        submitted_blocks: seq<SignedBeaconBlock>    
+    )  
+
+    function {:axiom} bn_get_fork_version(slot: Slot): Version
+
+    function {:axiom} bn_get_validator_index(bnState: BNState, state_id: Root, validator_id: BLSPubkey): (vi: Optional<ValidatorIndex>)
+    requires state_id in bnState.state_roots_of_imported_blocks
+
+    function {:axiom} bn_get_epoch_committees(bnState: BNState, state_id: Root, index: CommitteeIndex): (sv: seq<ValidatorIndex>) 
+    requires state_id in bnState.state_roots_of_imported_blocks   
+}
+
+module Att_BN_Axioms
+{
+    import opened Types 
+    import opened CommonFunctions
+
+    datatype BNState = BNState(
+        state_roots_of_imported_blocks: set<Root>,
+        attestations_submitted: seq<Attestation>    
+    )     
+
+    function {:axiom} bn_get_fork_version(slot: Slot): Version
+
+    function {:axiom} bn_get_validator_index(bnState: BNState, state_id: Root, validator_id: BLSPubkey): (vi: Optional<ValidatorIndex>)
+    requires state_id in bnState.state_roots_of_imported_blocks
+
+    function {:axiom} bn_get_epoch_committees(bnState: BNState, state_id: Root, index: CommitteeIndex): (sv: seq<ValidatorIndex>) 
+    requires state_id in bnState.state_roots_of_imported_blocks   
+}
